# 向量求导公式对照表

| 函数表达式                                                                          | 分母布局（Denominator Layout）                                                                  |
| :----------------------------------------------------------------------------- | :---------------------------------------------------------------------------------------- |
| $$y = a^T x$$                                                                  | $$\frac{\partial y}{\partial x} = a$$                                                     |
| $$y = a^T x + b$$                                                              | $$\frac{\partial y}{\partial x} = a$$                                                     |
| $$y = A x$$                                                                    | $$\frac{\partial y}{\partial x} = A^T$$                                                   |
| $$y = x^T A$$                                                                  | $$\frac{\partial y}{\partial x} = A$$                                                     |
| $$y = A x + b$$                                                                | $$\frac{\partial y}{\partial x} = A^T$$                                                   |
| $$y = x^T A x$$                                                                | $$\frac{\partial y}{\partial x} = (A + A^T)x$$                                            |
| $$y = c^T A x$$                                                                | $$\frac{\partial y}{\partial x} = A^T c$$                                                 |
| $$y = \|x\|_2^2 = x^T x$$                                                      | $$\frac{\partial y}{\partial x} = 2x$$                                                    |
| $$y = \|x\|_2 = x^T x$$                                                        | $$\frac{\partial y}{\partial x} = \frac{x}{\|x\|_2}$$                                     |
| $$y = x$$                                                                      | $$\frac{\partial y}{\partial x} = I_n$$                                                   |
| $$L = \sum_i \Big( -y_i \log(\hat{y}_i) - (1 - y_i)\log(1 - \hat{y}_i) \Big)$$ | $$\frac{\partial L}{\partial \hat{y}} = \frac{\hat{y} - y}{\hat{y} \odot (1 - \hat{y})}$$ |




